format-version: 1.2
data-version: 220927.1
remark: General comments for this file can go here
ontology: dpvis
property_value: default-relationship-id-prefix "dpvis" xsd:string

[Term]
id: dpvis:2DDensityPlot
name: 2D Density Plot
def: "Plot that shows the distribution of values of two numeric variables. It counts the number of observations by estimating them via e.g. a square or a kernel that is moved over the 2D space." []
comment: TODO is_a dpvis:DensityPlot?
is_a: dpvis:TwoDimVis
relationship: has_a dpvis:2DDensityPlotInputs ! 2D Density Plot Inputs
relationship: has_a dpvis:2DDensityPlotOutputs ! 2D Density Plot Outputs

[Term]
id: dpvis:2DDensityPlotInputs
name: 2D Density Plot Inputs
def: "Inputs of a [2DDensityPlot]" []
is_a: dpvis:Input ! Input
relationship: has_a dpvis:Colormap ! Colormap
relationship: has_a dpvis:ScalarsForColor ! Scalars for Color
relationship: has_a dpvis:ScalarsForX ! Scalars for X
relationship: has_a dpvis:ScalarsForY ! Scalars for Y

[Term]
id: dpvis:2DDensityPlotOutputs
name: 2D Density Plot Outputs
def: "Outputs of a [2DDensityPlot]" []
comment: "TODO: depending on kernel different outputs?"
is_a: dpvis:Output ! Output

[Term]
id: dpvis:Axis
name: Axis
def: "Line that specifies a value of an attribute." []
comment: "TODO different types of axis, e.g. numerical, categorical?"

[Term]
id: dpvis:AxisChart
name: Axis Chart
def: "Representation of relationships between different values in a coordinate system." []
comment: TODO subtypes for axischarts
is_a: dpvis:TwoDimVis

[Term]
id: dpvis:Bandwidth
name: The bandwidth of a [Kernelfunction] affects how “smooth” the resulting curve is. The lower the bandwidth the smaller is the considered neighborhood around an estimated point..

[Term]
id: dpvis:BarHistogram
name: Bar Histogram
def: "Show a univariate distribution by bars whose position and width corresponds to bins of the sample space and whose height corresponds to the data count there" []
is_a: dpvis:TwoDimVis
relationship: has_a dpvis:BarHistogramInputs ! Inputs of a Bar Histogram.
relationship: has_a dpvis:BarHistogramOutputs ! Outputs of a Bar Histogram.

[Term]
id: dpvis:BarHistogramInputs
name: Inputs of a Bar Histogram.
comment: "ScalarsForY should be estimate at position X"
is_a: dpvis:Input ! Input
relationship: has_a dpvis:Axis ! Axis
relationship: has_a dpvis:Colormap ! Colormap
relationship: has_a dpvis:NumberOfBins ! Integer specifying the amount of bins in which the data is to be seperated.
relationship: has_a dpvis:ScalarsForColor ! Scalars for Color
relationship: has_a dpvis:ScalarsForX ! Scalars for X
relationship: has_a dpvis:ScalarsForY ! Scalars for Y

[Term]
id: dpvis:BarHistogramOutputs
name: Outputs of a Bar Histogram.
is_a: dpvis:Output ! Output

[Term]
id: dpvis:BoxPlot
name: Box Plot
def: "Plot that shows the distribution of a numerical variable for one or several groups. The distribution is partitioned in its quartiles." []
comment: TODO is_a dpvis:DensityPlot?
is_a: dpvis:CartesianAxisChart ! Cartesian Axis Chart
relationship: has_a dpvis:BoxPlotInputs ! Box Plot Inputs
relationship: has_a dpvis:BoxPlotOutputs ! Box Plot Outputs

[Term]
id: dpvis:BoxPlotInputs
name: Box Plot Inputs
comment: TODO other inputs
is_a: dpvis:Input ! Input
relationship: has_a dpvis:Colormap ! Colormap
relationship: has_a dpvis:ScalarsForColor ! Scalars for Color

[Term]
id: dpvis:BoxPlotOutputs
name: Box Plot Outputs
is_a: dpvis:Output ! Output

[Term]
id: dpvis:BubbleChart
name: Bubble Chart
def: "Plot that can show 4D data through disks of varying size and color" []
comment: "Comment that is guaranteed to survive a load-save round-trip (contrary to the exclamation mark lines)"
is_a: dpvis:CartesianAxisChart ! Cartesian Axis Chart
relationship: has_a dpvis:BubbleChartInputs ! Bubble Chart Inputs
relationship: has_a dpvis:BubbleChartOutputs ! Bubble Chart Outputs
created_by: Christopher Kappe | ORCID: 0000-0003-4296-1734

[Term]
id: dpvis:BubbleChartInputs
name: Bubble Chart Inputs
comment: TODO add relationships if neccessary
is_a: dpvis:Input ! Input
relationship: has_a dpvis:ColoredCircles ! Colored Circles
relationship: has_a dpvis:Colormap ! Colormap
relationship: has_a dpvis:ScalarsForColor ! Scalars for Color

[Term]
id: dpvis:BubbleChartOutputs
name: Bubble Chart Outputs
is_a: dpvis:Output ! Output
relationship: has_a dpvis:ColoredCircles ! Colored Circles

[Term]
id: dpvis:CartesianAxisChart
name: Cartesian Axis Chart
def: "Representation of relationships between different values in a cartesian coordinate system." []
comment: TODO subtypes for axischarts
is_a: dpvis:AxisChart ! Axis Chart
relationship: has_a dpvis:Axis ! Axis

[Term]
id: dpvis:Categories
name: Categories
def: "Discrete labels or types with no implicit ordering." []
comment: Examples: colors, nations.

[Term]
id: dpvis:CirclePacking
name: Circle Packing
def: "Like a [Treemap] but with circles as areas. A circle represents a node and subnodes are the circles that are contained in it. Such Circle Packing depicts hierarchical structures, like the [Treemap] or [Dendogram]." []
is_a: dpvis:TwoDimVis
relationship: has_a dpvis:CirclePackingInputs ! Circle Packing Inputs
relationship: has_a dpvis:CirclePackingOutputs ! Circle Packing Outputs

[Term]
id: dpvis:CirclePackingInputs
name: Circle Packing Inputs
comment: TODO add relationships if neccessary
is_a: dpvis:Input ! Input
relationship: has_a dpvis:ColoredCircles ! Colored Circles
relationship: has_a dpvis:Colormap ! Colormap
relationship: has_a dpvis:ScalarsForColor ! Scalars for Color

[Term]
id: dpvis:CirclePackingOutputs
name: Circle Packing Outputs
is_a: dpvis:Output ! Output
relationship: has_a dpvis:ColoredCircles ! Colored Circles

[Term]
id: dpvis:CircularAreaChart
name: Circular Area Chart
def: "Similar to a [LineChart] but the area under the line is filled and the domain is mapped to 360° (and the chart drawn accordingly) with axes for the codomain repeated e.g. every 45°" []
is_a: dpvis:TwoDimVis

[Term]
id: dpvis:ColoredCircles
name: Colored Circles
comment: TODO Continue
relationship: has_a dpvis:Colormap ! Colormap
relationship: has_a dpvis:Radius ! Radius
relationship: has_a dpvis:ScalarsForColor ! Scalars for Color

[Term]
id: dpvis:Colormap
name: Colormap
def: "Maps values or value ranges to a color." []

[Term]
id: dpvis:Correlogram
name: Correlogram
def: "Visualizes the pairwise relationship between two numeric variables of a matrix. The correlation of each pair can be visualized by a [Scatterplot] or a symbolic representation of its value, e.g. bubble. Options for the diagonal are [Histogram] or [DensityPlot]." []
comment: How to reference a list of possible options?
is_a: dpvis:TwoDimVis
relationship: has_a dpvis:CorrelogramInputs ! Correlogram Inputs
relationship: has_a dpvis:CorrelogramOutputs ! Correlogram Outputs

[Term]
id: dpvis:CorrelogramInputs
name: Correlogram Inputs
comment: "TODO relationships depend on how each pair is visualized e.g. scatterplotinputs for a scatterplot"
is_a: dpvis:Input ! Input

[Term]
id: dpvis:CorrelogramOutputs
name: Correlogram Outputs
is_a: dpvis:Output ! Output
relationship: has_a dpvis:ColoredCircles ! Colored Circles

[Term]
id: dpvis:Dendogram
name: Dendogram
def: "A tree that depicts data in a hierarchical structure. Datasets can be either hierarchical themselves or numeric data matrix to compute distances between the data points (clustering)." []
comment: TODO How to correctly reference clustering?
is_a: dpvis:TwoDimVis
relationship: has_a dpvis:DendogramInputs ! Dendogram Inputs
relationship: has_a dpvis:DendogramOutputs ! Dendogram Outputs

[Term]
id: dpvis:DendogramInputs
name: Dendogram Inputs
comment: TODO relationship
is_a: dpvis:Input ! Input

[Term]
id: dpvis:DendogramOutputs
name: Dendogram Outputs
is_a: dpvis:Output ! Output
relationship: has_a dpvis:ColoredCircles ! Colored Circles

[Term]
id: dpvis:DensityPlot
name: Density Plot
def: "Shows the distribution of a numeric variable. Very close to a histogram." []
comment: TODO is_a dpvis:DensityPlot?
is_a: dpvis:TwoDimVis
relationship: has_a dpvis:Bandwidth ! The bandwidth of a [Kernelfunction] affects how “smooth” the resulting curve is. The lower the bandwidth the smaller is the considered neighborhood around an estimated point..
relationship: has_a dpvis:DensityPlotInputs ! Density Plot Inputs
relationship: has_a dpvis:DensityPlotOutputs ! Density Plot Outputs
relationship: has_a dpvis:Kernelfunction ! Function that estimates the density of points within a region by weighting the distances.

[Term]
id: dpvis:DensityPlotInputs
name: Density Plot Inputs
def: "Inputs of a [DensityPlot]" []
comment: TODO add relationships if neccessary
is_a: dpvis:Input ! Input
relationship: has_a dpvis:Colormap ! Colormap
relationship: has_a dpvis:ScalarsForColor ! Scalars for Color
relationship: has_a dpvis:ScalarsForX ! Scalars for X
relationship: has_a dpvis:ScalarsForY ! Scalars for Y

[Term]
id: dpvis:DensityPlotOutputs
name: Density Plot Outputs
def: "Outputs of a [DensityPlot]" []
comment: "TODO: depending on kernel different outputs?"
is_a: dpvis:Output ! Output
relationship: has_a dpvis:ScalarsForX ! Scalars for X
relationship: has_a dpvis:ScalarsForY ! Scalars for Y

[Term]
id: dpvis:DotPlot
name: Dot Plot
def: "Matrix visualization to compare two (bio) sequences by drawing black dots in fields that match" []
is_a: dpvis:Heatmap ! Heatmap

[Term]
id: dpvis:Doughnut
name: Doughnut
def: "Basically a [PieChart] with a hole inside. The sections of the Doughnut represent the relative size of their value." []
is_a: dpvis:TwoDimVis

[Term]
id: dpvis:Edge
name: Edge
def: "Connects one [Node] with another one in a [Graph]. Can either be directed or undirected." []

[Term]
id: dpvis:Edges
name: Edges
def: "A set of [Edge]s." []

[Term]
id: dpvis:Graph
name: Graph
def: "Representation of relationships between different nodes through edges. Graphs can be directed or undirected." []
comment: TODO subtypes for graphs
is_a: dpvis:TwoDimVis
relationship: has_a dpvis:Nodes
relationship: has_a dpvis:Edges

[Term]
id: dpvis:Heatmap
name: Heatmap
def: "Matrix visualization to compare two sequences by coloring the fields e.g. w.r.t. some similarity" []
is_a: dpvis:TwoDimVis

[Term]
id: dpvis:HoriBarChart
name: Horizontal Bar Chart
def: "Chart that has a horizontal bar for every (named) scalar variable" []
is_a: dpvis:AxisChart ! Axis Chart

[Term]
id: dpvis:Input
name: Input
def: "Input of a plot" []

[Term]
id: dpvis:Kernelfunction
name: Function that estimates the density of points within a region by weighting the distances.

[Term]
id: dpvis:LineChart
name: Line Chart
def: "Chart that shows a line for one or more scalar variables that are defined on a continuous 1D domain" []
is_a: dpvis:AxisChart ! Axis Chart
relationship: has_a dpvis:Axis ! Axis

[Term]
id: dpvis:LineHistogram
name: Line Histogram
def: "Show a univariate distribution by a continuous line whose height is determined by the probability" []
is_a: dpvis:AxisChart ! Axis Chart

[Term]
id: dpvis:Lollipop
name: Lollipop
def: "Is a special kind of [BarChart], where instead of the bar we have a line and a dot." []
is_a: dpvis:TwoDimVis

[Term]
id: dpvis:Node
name: Node
def: "A node represents an object or data item. Special nodes are the root and the leaves." []

[Term]
id: dpvis:Nodes
name: Nodes
def: "A set of [Node]s." []

[Term]
id: dpvis:NumberOfBins
name: Integer specifying the amount of bins in which the data is to be seperated.

[Term]
id: dpvis:Ordinals
name: Ordinal data
def: "Discrete data with an implicit ordering." []
comment: Examples: grades, ranking.

[Term]
id: dpvis:Output
name: Output
def: "Output of a plot" []

[Term]
id: dpvis:PCA
name: PCA
def: "Visualizes the pairwise relationship between two numeric variables of a matrix. The correlation of each pair can be visualized by a [Scatterplot] or a symbolic representation of its value, e.g. bubble. Options for the diagonal are [Histogram] or [DensityPlot]." []
comment: TODO How to reference a list of possible options?
is_a: dpvis:TwoDimVis

[Term]
id: dpvis:ParallelCoordinates
name: Parallel Coordinates
def: "Comparison of data points through their variables. Vertical axis represent numeric variables and can have different scales. Each data point is plotted as a line that connects the values on each axis." []
comment: Like a [SpiderChart], but with cartesian coordinates.
is_a: dpvis:TwoDimVis

[Term]
id: dpvis:PieChart
name: Pie Chart
def: "A circle whose sections (or slices) are represent a relative size" []
is_a: dpvis:TwoDimVis

[Term]
id: dpvis:Quartiles
name: Quartiles
def: "A quantile that devides the number of data points into four parts of equal size. The data has to be ordered in ascending order before being partitioned." []
comment: TODO add relationships if there are any. Is only a definition so far.

[Term]
id: dpvis:RadialAxisChart
name: Radial Axis Chart
def: "Representation of relationships between different values in a coordinate system." []
comment: TODO subtypes for axischarts
is_a: dpvis:AxisChart ! Axis Chart
relationship: has_a dpvis:Axis ! Axis

[Term]
id: dpvis:Radius
name: Radius
def: "Number that defines the size of a circle" []
is_a: dpvis:Scalar ! Scalar

[Term]
id: dpvis:RidgelinePlot
name: Ridgeline plot
def: "Similar to [StackedAreaChart] but displaced around a central axis and with rounded edges to give it an organic appearance. Distributions can be visualized by [LineHistogram] or [DensityPlot] which are aligned on horizontal axis and slightly overlap one another." []
comment: TODO is_a: dpvis:StackedAreaChart ?
synonym: "Joyplot" RELATED []
is_a: dpvis:TwoDimVis

[Term]
id: dpvis:SankeyDiagram
name: Sankey Diagram
def: "Representation of flows over links. The width of a flow represents its importance." []
comment: "Alluvial diagram is a sub category. TODO: term for alluvial diagram or delete comment."
is_a: dpvis:TwoDimVis

[Term]
id: dpvis:Scalar
name: Scalar
def: "Real number as in the mathematical sense" []
comment: Should maybe be called Number or Real

[Term]
id: dpvis:Scalars
name: Scalars
def: "Finite set of scalars (real numbers)" []

[Term]
id: dpvis:ScalarsForColor
name: Scalars for Color
def: "Scalars that are intended to be mapped to colors" []
is_a: dpvis:Scalars ! Scalars

[Term]
id: dpvis:ScalarsForX
name: Scalars for X
def: "Scalars that are intended to be mapped to x-coordinates" []
is_a: dpvis:Scalars ! Scalars

[Term]
id: dpvis:ScalarsForY
name: Scalars for Y
def: "Scalars that are intended to be mapped to y-coordinates" []
is_a: dpvis:Scalars ! Scalars

[Term]
id: dpvis:Scatterplot
name: Scatterplot
def: "Plot that shows 2D points that may be colored individually" []
comment: NOTE Do we need the following relations explicitly?
is_a: dpvis:BubbleChart ! Bubble Chart
relationship: has_a dpvis:ScatterplotInputs ! Scatterplot Inputs
relationship: has_a dpvis:ScatterplotOutputs ! Scatterplot Outputs

[Term]
id: dpvis:ScatterplotInputs
name: Scatterplot Inputs
def: "Inputs of a [Scatterplot]" []
comment: This includes "small" stuff like parameters and "large" stuff like datasets
is_a: dpvis:Input ! Input
relationship: has_a dpvis:Colormap ! Colormap
relationship: has_a dpvis:Radius ! Radius
relationship: has_a dpvis:ScalarsForColor ! Scalars for Color
relationship: has_a dpvis:ScalarsForX ! Scalars for X
relationship: has_a dpvis:ScalarsForY ! Scalars for Y

[Term]
id: dpvis:ScatterplotOutputs
name: Scatterplot Outputs
def: "Outputs of a [Scatterplot]" []
is_a: dpvis:Output ! Output
relationship: has_a dpvis:ColoredCircles ! Colored Circles

[Term]
id: dpvis:SpiderChart
name: Spider Chart
def: "Comparison of data points through their variables. Each axis represents a numeric variable and the axis are joint in the center of the plot. Each data point is plotted as a line that connects the values on each axis." []
comment: Like [ParallelCoordinates], but with circular layout.
synonym: "Radar chart" RELATED []
synonym: "Web chart" RELATED []
is_a: dpvis:Graph ! Graph

[Term]
id: dpvis:Stacked100AreaChart
name: Stacked 100% Area Chart
def: "Like a [StackedAreaChart] but the accumalated height at each sample is normalized to 100%" []
is_a: dpvis:AxisChart ! Axis Chart

[Term]
id: dpvis:Stacked100BarChart
name: Stacked 100% Bar Chart
def: "Like a [StackedBarChart] but every bar has the same height s.t. the proportions of the categories can easily be compared across the bars" []
is_a: dpvis:AxisChart ! Axis Chart

[Term]
id: dpvis:StackedAreaChart
name: Stacked Area Chart
def: "Similar to a [LineChart] but there are always at least two lines and their height is given by stacking and the area under the lines is filled accordingly" []
is_a: dpvis:AxisChart ! Axis Chart

[Term]
id: dpvis:StackedBarChart
name: Stacked Bar Chart
def: "Like a [VertBarChart] but the scalar variables depend on an additional dimension (typically a set of categories)" []
is_a: dpvis:AxisChart ! Axis Chart

[Term]
id: dpvis:Streamgraph
name: Streamgraph
def: "Similar to [StackedAreaChart] but displaced around a central axis and with rounded edges to give it an organic appearance." []
comment: TODO is_a: dpvis:StackedAreaChart ?
is_a: dpvis:TwoDimVis

[Term]
id: dpvis:Sunburst
name: Sunburst
def: "Basically a [PieChart] or [Doughnut] with multiple levels to depict hierarchies." []
synonym: "multi-level pie chart" RELATED []
synonym: "Radial Treemap" RELATED []
is_a: dpvis:TwoDimVis

[Term]
id: dpvis:Treemap
name: Treemap
def: "Visualization of a tree data structure whose nodes are represented by nested rectangles whose area reflects some variable." []
is_a: dpvis:TwoDimVis

[Term]
id: dpvis:VarWiBarChart
name: Variable-width Bar Chart
def: "Like a [VertBarChart] but takes 2D variables and the width of a bar represents the value in the second dimension" []
is_a: dpvis:AxisChart ! Axis Chart

[Term]
id: dpvis:Venn
name: Venn Diagram
def: "Shows logical relationships between different groups. Groups are represented by circles which size represent the importance of the respective group. Intersection of two circles and the size of the intersection represent how much the two groups intersect with one another." []
synonym: "logic diagram" RELATED []
synonym: "primary diagram" RELATED []
synonym: "set diagram" RELATED []
is_a: dpvis:TwoDimVis

[Term]
id: dpvis:VertBarChart
name: Vertical Bar Chart
def: "Chart that has a vertical bar for every (named) scalar variable" []
is_a: dpvis:AxisChart ! Axis Chart

[Term]
id: dpvis:Violin
name: Violin Plot
def: "Plot that shows the distribution of a numerical variable for one or several groups. It is similar to a [BoxPlot], but additionally shows the probability density." []
comment: TODO is_a dpvis:DensityPlot?
is_a: dpvis:TwoDimVis

[Term]
id: dpvis:WaterfallChart
name: Waterfall Chart
def: "Similar to a [VertBarChart] where the x-axis represents time or categories and the bars start at the top or bottom of its predecessor, growing up or down depending on the sign of the depicted variable" []
comment: "Aka. flying bricks chart or Mario chart"
is_a: dpvis:TwoDimVis

[Term]
id: dpvis:Wordcloud
name: Wordcloud
def: "Generates an image with words where the size or color enocdes the importance of each word. Allows to quickly perceive the most prominent terms." []
is_a: dpvis:TwoDimVis

[Typedef]
id: dpvis:has_a
name: Has
def: "The typical supplement to [global:is_a]. Very generic composition relation. If *a* has_a *b*, *b* is some kind of attribute, property or possession of *a*." []
comment: "Edge (i.e. relation) type; the unintuitive name "Typedef" for historical reasons."

