format-version: 1.4
data-version: 220927.1
ontology: dpvis
default-relationship-id-prefix: dpvis
remark: General comments for this file can go here


[Typedef]
id: dpvis:has_a
name: Has
def: "The typical supplement to [global:is_a]. Very generic composition relation. If *a* has_a *b*, *b* is some kind of attribute, property or possession of *a*."
comment: "Edge (i.e. relation) type; the unintuitive name \"Typedef\" for historical reasons."


[Term]
id: dpvis:BubbleChart
name: Bubble Chart
def: "Plot that can show 4D data through disks of varying size and color"
is_a: dpvis:TwoDimVis
comment: "Comment that is guaranteed to survive a load-save round-trip (contrary to the exclamation mark lines)"
created_by: Christopher Kappe | ORCID: 0000-0003-4296-1734



[Term]
id: dpvis:ScalarsForX
name: Scalars for X
def: "Scalars that are intended to be mapped to x-coordinates"
is_a: dpvis:Scalars

[Term]
id: dpvis:ScalarsForY
name: Scalars for Y
def: "Scalars that are intended to be mapped to y-coordinates"
is_a: dpvis:Scalars

[Term]
id: dpvis:ScalarsForColor
name: Scalars for Color
def: "Scalars that are intended to be mapped to colors"
is_a: dpvis:Scalars

[Term]
id: dpvis:Scalars
name:  Scalars
def: "Finite set of scalars (real numbers)"

[Term]
id: dpvis:Radius
name: Radius
def: "Number that defines the size of a circle"
is_a: dpvis:Scalar

[Term]
id: dpvis:Scalar
name: Scalar
def: "Real number as in the mathematical sense"
comment: Should maybe be called Number or Real

[Term]
id: dpvis:ScatterplotInputs
name: Scatterplot Inputs
def: "Inputs of a [Scatterplot]"
comment: This includes "small" stuff like parameters and "large" stuff like datasets
relationship: has_a dpvis:ScalarsForX
relationship: has_a dpvis:ScalarsForY
relationship: has_a dpvis:ScalarsForColor
relationship: has_a dpvis:Colormap
comment: "We expect implementations to be able to deal with zero or one color"
relationship: has_a dpvis:Radius

[Term]
id: dpvis:ColoredCircles
name: Colored Circles
comment: TODO Continue

[Term]
id: dpvis:ScatterplotOutputs
name: Scatterplot Outputs
def: "Outputs of a [Scatterplot]"
relationship: has_a dpvis:ColoredCircles

[Term]
id: dpvis:Scatterplot
name: Scatterplot
def: "Plot that shows 2D points that may be colored individually"
is_a: dpvis:BubbleChart
comment: NOTE Do we need the following relations explicitly?
relationship: has_a dpvis:ScatterplotInputs
relationship: has_a dpvis:ScatterplotOutputs

[Term]
id: dpvis:Heatmap
name: Heatmap
def: "Matrix visualization to compare two sequences by coloring the fields e.g. w.r.t. some similarity"
is_a: dpvis:TwoDimVis

[Term]
id: dpvis:DotPlot
name: Dot Plot
def: "Matrix visualization to compare two (bio) sequences by drawing black dots in fields that match"
is_a: dpvis:Heatmap


[Term]
id: dpvis:VertBarChart
name: Vertical Bar Chart
def: "Chart that has a vertical bar for every (named) scalar variable"

[Term]
id: dpvis:HoriBarChart
name: Horizontal Bar Chart
def: "Chart that has a horizontal bar for every (named) scalar variable"

[Term]
id: dpvis:VarWiBarChart
name: Variable-width Bar Chart
def: "Like a [VertBarChart] but takes 2D variables and the width of a bar represents the value in the second dimension"

[Term]
id: dpvis:StackedBarChart
name: Stacked Bar Chart
def: "Like a [VertBarChart] but the scalar variables depend on an additional dimension (typically a set of categories)"

[Term]
id: dpvis:Stacked100BarChart
name: Stacked 100% Bar Chart
def: "Like a [StackedBarChart] but every bar has the same height s.t. the proportions of the categories can easily be compared across the bars"


[Term]
id: dpvis:LineChart
name: Line Chart
def: "Chart that shows a line for one or more scalar variables that are defined on a continuous 1D domain"

[Term]
id: dpvis:StackedAreaChart
name: Stacked Area Chart
def: "Similar to a [LineChart] but there are always at least two lines and their height is given by stacking and the area under the lines is filled accordingly"

[Term]
id: dpvis:Stacked100AreaChart
name: Stacked 100% Area Chart
def: "Like a [StackedAreaChart] but the accumalated height at each sample is normalized to 100%"

[Term]
id: dpvis:CircularAreaChart
name: Circular Area Chart
def: "Similar to a [LineChart] but the area under the line is filled and the domain is mapped to 360° (and the chart drawn accordingly) with axes for the codomain repeated e.g. every 45°"


[Term]
id: dpvis:BarHistogram
name: Bar Histogram
def: "Show a univariate distribution by bars whose position and width corresponds to bins of the sample space and whose height corresponds to the data count there"

[Term]
id: dpvis:LineHistogram
name: Line Histogram
def: "Show a univariate distribution by a continuous line whose height is determined by the probability"


[Term]
id: dpvis:PieChart
name: Pie Chart
def: "A circle whose sections (or slices) are represent a relative size"


[Term]
id: dpvis:Treemap
name: Treemap
def: "Visualization of a tree data structure whose nodes are represented by nested rectangles whose area reflects some variable."


[Term]
id: dpvis:WaterfallChart
name: Waterfall Chart
def: "Similar to a [VertBarChart] where the x-axis represents time or categories and the bars start at the top or bottom of its predecessor, growing up or down depending on the sign of the depicted variable
comment: "Aka. flying bricks chart or Mario chart"

[Term]
id: dpvis:Categories
name: Categories
def: "Discrete labels or types with no implicit ordering."
comment: Examples: colors, nations.

[Term]
id: dpvis:Ordinals
name: Ordinal data
def: "Discrete data with an implicit ordering."
comment: Examples: grades, ranking.

[Term]
id: dpvis:DensityPlot
name: Density Plot
def: "Plot that shows the distribution of a numeric variable."
comment: TODO is_a DensityPlot?

[Term]
id: dpvis:DensityPlotInputs
name: Density Plot Inputs
def: "Inputs of a [DensityPlot]"
comment: TODO depending on dimensionality more scalars are needed
relationship: has_a dpvis:ScalarsForX
relationship: has_a dpvis:ScalarsForY
relationship: has_a dpvis:ScalarsForColor
comment: "We expect implementations to be able to deal with zero or one color"

[Term]
id: dpvis:2dDensityPlot
name: 2D Density Plot
def: "Plot that shows the distribution of values of two numeric variables. It counts the number of observations by estimating them via e.g. a square or a kernel that is moved over the 2D space."
is_a: dpvis:TwoDimVis
comment: TODO is_a dpvis:DensityPlot?

[Term]
id: dpvis:2dDensityPlotInputs
name: 2D Density Plot Inputs
def: "Inputs of a [2dDensityPlot]"
relationship: has_a dpvis:ScalarsForX
relationship: has_a dpvis:ScalarsForY
relationship: has_a dpvis:ScalarsForColor
relationship: has_a dpvis:Colormap
comment: "We expect implementations to be able to deal with zero or one color"

[Term]
id: dpvis:2dDensityPlotOutputs
name: 2D Density Plot Outputs
def: "Outputs of a [2dDensityPlot]"
relationship: has_a dpvis:ScalarsForX
relationship: has_a dpvis:ScalarsForY
comment: "We expect implementations to be able to deal with zero or one color"
comment: "TODO: depending on kernel different outputs?"

[Term]
id: dpvis:Violin
name: Violin Plot
def: "Plot that shows the distribution of a numerical variable for one or several groups. It is similar to a [BoxPlot], but additionally shows the probability density."
is_a: dpvis:TwoDimVis
comment: TODO is_a dpvis:DensityPlot? 

[Term]
id: dpvis:BoxPlot
name: Box Plot
def: "Plot that shows the distribution of a numerical variable for one or several groups. The distribution is partitioned in its quartiles."
is_a: dpvis:TwoDimVis
comment: TODO is_a dpvis:DensityPlot?

[Term]
id: dpvis:Quartiles
name: Quartiles
def: "A quantile that devides the number of data points into four parts of equal size. The data has to be ordered in ascending order before being partitioned."
comment: TODO add relationships if there are any. Is only a definition so far.

[Term]
id: dpvis:Streamgraph
name: Streamgraph
def: "Similar to [StackedAreaChart] but displaced around a central axis and with rounded edges to give it an organic appearance."
is_a: dpvis:TwoDimVis
comment: TODO is_a: dpvis:StackedAreaChart ?

[Term]
id: dpvis:RidgelinePlot 
name: Ridgeline plot 
def: "Similar to [StackedAreaChart] but displaced around a central axis and with rounded edges to give it an organic appearance. Distributions can be visualized by [LineHistogram] or [DensityPlot] which are aligned on horizontal axis and slightly overlap one another."
is_a: dpvis:TwoDimVis
comment: TODO is_a: dpvis:StackedAreaChart ?
synonym: Joyplot

[Term]
id: dpvis:Correlogram  
name: Correlogram
def: "Visualizes the pairwise relationship between two numeric variables of a matrix. The correlation of each pair can be visualized by a [Scatterplot] or a symbolic representation of its value, e.g. bubble. Options for the diagonal are [Histogram] or [DensityPlot]."
is_a: dpvis:TwoDimVis
comment: How to reference a list of possible options?

[Term]
id: dpvis:PCA  
name: PCA
def: "Visualizes the pairwise relationship between two numeric variables of a matrix. The correlation of each pair can be visualized by a [Scatterplot] or a symbolic representation of its value, e.g. bubble. Options for the diagonal are [Histogram] or [DensityPlot]."
is_a: dpvis:TwoDimVis
comment: TODO How to reference a list of possible options?

[Term]
id: dpvis:Dendogram  
name: Dendogram
def: "A tree that depicts data in a hierarchical structure. Datasets can be either hierarchical themselves or numeric data matrix to compute distances between the data points (clustering)."
is_a: dpvis:TwoDimVis
comment: TODO How to correctly reference clustering?

[Term]
id: dpvis:Lollipop  
name: Lollipop
def: "Is a special kind of [BarChart], where instead of the bar we have a line and a dot."
is_a: dpvis:TwoDimVis

[Term]
id: dpvis:Wordcloud  
name: Wordcloud
def: "Generates an image with words where the size or color enocdes the importance of each word. Allows to quickly perceive the most prominent terms."
is_a: dpvis:TwoDimVis

[Term]
id: dpvis:Doughnut  
name: Doughnut
def: "Basically a [PieChart] with a hole inside. The sections of the Doughnut represent the relative size of their value."
is_a: dpvis:TwoDimVis

[Term]
id: dpvis:CirclePacking  
name: Circle Packing
def: "Like a [Treemap] but with circles as areas. A circle represents a node and subnodes are the circles that are contained in it. Such Circle Packing depicts hierarchical structures, like the [Treemap] or [Dendogram]."
is_a: dpvis:TwoDimVis

[Term]
id: dpvis:Venn  
name: Venn Diagram
def: "Shows logical relationships between different groups. Groups are represented by circles which size represent the importance of the respective group. Intersection of two circles and the size of the intersection represent how much the two groups intersect with one another."
is_a: dpvis:TwoDimVis
synonym: primary diagram
synonym: set diagram
synonym: logic diagram

[Term]
id: dpvis:Sunburst  
name: Sunburst
def: "Basically a [PieChart] or [Doughnut] with multiple levels to depict hierarchies."
is_a: dpvis:TwoDimVis
synonym: multi-level pie chart
synonym: Radial Treemap

[Term]
id: dpvis:ParallelCoordinates  
name: Parallel Coordinates
def: "Comparison of data points through their variables. Vertical axis represent numeric variables and can have different scales. Each data point is plotted as a line that connects the values on each axis."
is_a: dpvis:TwoDimVis
comment: Like a [SpiderChart], but with cartesian coordinates.

[Term]
id: dpvis:SpiderChart  
name: Spider Chart
def: "Comparison of data points through their variables. Each axis represents a numeric variable and the axis are joint in the center of the plot. Each data point is plotted as a line that connects the values on each axis."
is_a: dpvis:TwoDimVis
comment: Like [ParallelCoordinates], but with circular layout.
synonym: Web chart
synonym: Radar chart

[Term]
id: dpvis:SankeyDiagram
name: Sankey Diagram
def: "Representation of flows over links. The width of a flow represents its importance."
is_a: dpvis:TwoDimVis
comment: Alluvial diagram is a sub category. TODO: term for alluvial diagram or delete comment.